src/Dafny/util/arith.dfy
@@ -1,0 +1,21 @@
+module Arith {
+  lemma div_mod_split(x: nat, k: nat)
+      requires 0 < k
+      ensures x == (x/k)*k + x%k
+  {
+  }
+
+  lemma div_mod_bound(x1: nat, x2: nat, x1_bound: nat, k:nat)
+      requires 0 < k
+      requires x1 < x1_bound
+      requires x2 < k
+      ensures x1*k + x2 < k*x1_bound
+  {
+      assert x1 <= x1_bound-1;
+      calc {
+          x1 * k;
+          <= (x1_bound-1)*k;
+          == x1_bound*k-k;
+      }
+  }
+}
